spec/arch/msp430/mem.i.dfy
@@ -1,697 +1,697 @@
-include "stack.i.dfy"
+// include "stack.i.dfy"
 
-module mem {
-  import opened integers
-  import opened flat
-  import opened stack
+// module mem {
+//   import opened integers
+//   import opened flat
+//   import opened stack
 
-  datatype entry_t = 
-    | W16(w16: uint16)
-    | B16(b16: seq<uint16>)
+//   datatype entry_t = 
+//     | W16(w16: uint16)
+//     | B16(b16: seq<uint16>)
 
-  type heap_t = map<int, entry_t>
+//   type heap_t = map<int, entry_t>
 
-  function heap_b16_index_ptr(ptr: nat, i: nat): nat
-  {
-    ptr + i * 2
-  }
+//   function heap_b16_index_ptr(ptr: nat, i: nat): nat
+//   {
+//     ptr + i * 2
+//   }
 
-  predicate heap_b16_ptr_valid(heap: heap_t, base_ptr: nat)
-  {
-    && ptr_admissible_16(base_ptr)
-    && base_ptr in heap
-    && heap[base_ptr].B16?
-    && var len := |heap[base_ptr].b16|;
-    //  the buffer is not empty
-    && len != 0
-    // end of buffer is in bound
-    && ptr_admissible_16(heap_b16_index_ptr(base_ptr, len - 1))
-  }
+//   predicate heap_b16_ptr_valid(heap: heap_t, base_ptr: nat)
+//   {
+//     && ptr_admissible_16(base_ptr)
+//     && base_ptr in heap
+//     && heap[base_ptr].B16?
+//     && var len := |heap[base_ptr].b16|;
+//     //  the buffer is not empty
+//     && len != 0
+//     // end of buffer is in bound
+//     && ptr_admissible_16(heap_b16_index_ptr(base_ptr, len - 1))
+//   }
 
-  // this holds for each uint16 in a b16 heaplet entry
-  predicate heap_16_inv(heap: heap_t, flat: flat_t, base_ptr: nat, i: nat)
-    requires heap_b16_ptr_valid(heap, base_ptr)
-    requires i < |heap[base_ptr].b16|
-  {
-    var ptr := heap_b16_index_ptr(base_ptr, i);
-    // ptr points to some uint16, which has 8 base words uint16
-    && flat_ptr_valid_16(flat, ptr)
-    && flat_read_16(flat, ptr) == heap[base_ptr].b16[i]
-    // disjointness
-    && (i != 0 ==> ptr !in heap)
-    && !in_stack_addr_range(ptr + 0)
-    && ptr + 0 !in heap
-  }
+//   // this holds for each uint16 in a b16 heaplet entry
+//   predicate heap_16_inv(heap: heap_t, flat: flat_t, base_ptr: nat, i: nat)
+//     requires heap_b16_ptr_valid(heap, base_ptr)
+//     requires i < |heap[base_ptr].b16|
+//   {
+//     var ptr := heap_b16_index_ptr(base_ptr, i);
+//     // ptr points to some uint16, which has 8 base words uint16
+//     && flat_ptr_valid_16(flat, ptr)
+//     && flat_read_16(flat, ptr) == heap[base_ptr].b16[i]
+//     // disjointness
+//     && (i != 0 ==> ptr !in heap)
+//     && !in_stack_addr_range(ptr + 0)
+//     && ptr + 0 !in heap
+//   }
 
-  // this holds for each b16 heaplet entry
-  predicate heap_b16_inv(heap: heap_t, flat: flat_t, base_ptr: nat)
-    requires heap_b16_ptr_valid(heap, base_ptr)
-  {
-    forall i | 0 <= i < |heap[base_ptr].b16| ::
-      heap_16_inv(heap, flat, base_ptr, i)
-  }
+//   // this holds for each b16 heaplet entry
+//   predicate heap_b16_inv(heap: heap_t, flat: flat_t, base_ptr: nat)
+//     requires heap_b16_ptr_valid(heap, base_ptr)
+//   {
+//     forall i | 0 <= i < |heap[base_ptr].b16| ::
+//       heap_16_inv(heap, flat, base_ptr, i)
+//   }
 
-  function heap_b16_read(heap: heap_t, iter: b16_iter): uint16
-    requires b16_iter_safe(heap, iter)
-  {
-    var buff := heap[iter.base_ptr].b16;
-    buff[iter.index]
-  }
+//   function heap_b16_read(heap: heap_t, iter: b16_iter): uint16
+//     requires b16_iter_safe(heap, iter)
+//   {
+//     var buff := heap[iter.base_ptr].b16;
+//     buff[iter.index]
+//   }
 
-  function heap_b16_write(heap: heap_t, iter: b16_iter, value: uint16): heap_t
-    requires b16_iter_safe(heap, iter)
-  {
-    var buff := heap[iter.base_ptr].b16;
-    var new_buff := buff[iter.index := value];
-    heap[iter.base_ptr := B16(new_buff)]
-  }
+//   function heap_b16_write(heap: heap_t, iter: b16_iter, value: uint16): heap_t
+//     requires b16_iter_safe(heap, iter)
+//   {
+//     var buff := heap[iter.base_ptr].b16;
+//     var new_buff := buff[iter.index := value];
+//     heap[iter.base_ptr := B16(new_buff)]
+//   }
 
 
-  // iterator for buffer entries
-  datatype b16_iter = b16_iter_cons(base_ptr: nat, index: nat, buff: seq<uint16>)
-  {
-    function cur_ptr(): nat {
-      heap_b16_index_ptr(base_ptr, index)
-    }
-  }
+//   // iterator for buffer entries
+//   datatype b16_iter = b16_iter_cons(base_ptr: nat, index: nat, buff: seq<uint16>)
+//   {
+//     function cur_ptr(): nat {
+//       heap_b16_index_ptr(base_ptr, index)
+//     }
+//   }
 
-  function b16_iter_load_next(iter: b16_iter, inc: bool): b16_iter
-  {
-    iter.(index := if inc then iter.index + 1 else iter.index)
-  }
+//   function b16_iter_load_next(iter: b16_iter, inc: bool): b16_iter
+//   {
+//     iter.(index := if inc then iter.index + 1 else iter.index)
+//   }
 
-  function b16_iter_load_prev(iter: b16_iter): b16_iter
-  {
-    if iter.index == 0 then iter else iter.(index := iter.index - 1)
-  }
+//   function b16_iter_load_prev(iter: b16_iter): b16_iter
+//   {
+//     if iter.index == 0 then iter else iter.(index := iter.index - 1)
+//   }
 
-  function b16_iter_store_next(iter: b16_iter, value: uint16, inc: bool): b16_iter
-    requires iter.index < |iter.buff|
-  {
-      iter.(index := if inc then iter.index + 1 else iter.index)
-          .(buff := iter.buff[iter.index := value])
-  }
+//   function b16_iter_store_next(iter: b16_iter, value: uint16, inc: bool): b16_iter
+//     requires iter.index < |iter.buff|
+//   {
+//       iter.(index := if inc then iter.index + 1 else iter.index)
+//           .(buff := iter.buff[iter.index := value])
+//   }
 
-  predicate b16_iter_inv(heap: heap_t, iter: b16_iter)
-  {
-    var base_ptr := iter.base_ptr;
-    // base_ptr points to a valid buffer
-    && heap_b16_ptr_valid(heap, base_ptr)
-    // ptr is correct
-    && iter.cur_ptr() == heap_b16_index_ptr(base_ptr, iter.index)
-    // the view is consistent with heap
-    && heap[base_ptr].b16 == iter.buff
-    // the index is within bound (or at end)
-    && iter.index <= |iter.buff|
-  }
+//   predicate b16_iter_inv(heap: heap_t, iter: b16_iter)
+//   {
+//     var base_ptr := iter.base_ptr;
+//     // base_ptr points to a valid buffer
+//     && heap_b16_ptr_valid(heap, base_ptr)
+//     // ptr is correct
+//     && iter.cur_ptr() == heap_b16_index_ptr(base_ptr, iter.index)
+//     // the view is consistent with heap
+//     && heap[base_ptr].b16 == iter.buff
+//     // the index is within bound (or at end)
+//     && iter.index <= |iter.buff|
+//   }
 
-  predicate b16_iter_safe(heap: heap_t, iter: b16_iter)
-  {
-    && b16_iter_inv(heap, iter)
-    // tighter constraint so we can dereference
-    && iter.index < |iter.buff|
-  }
+//   predicate b16_iter_safe(heap: heap_t, iter: b16_iter)
+//   {
+//     && b16_iter_inv(heap, iter)
+//     // tighter constraint so we can dereference
+//     && iter.index < |iter.buff|
+//   }
 
-  // valid pointer for W16 heaplet entry
-  predicate heap_w16_ptr_valid(heap: heap_t, base_ptr: nat)
-  {
-    && ptr_admissible_16(base_ptr)
-    && base_ptr in heap
-    && heap[base_ptr].W16?
-  }
+//   // valid pointer for W16 heaplet entry
+//   predicate heap_w16_ptr_valid(heap: heap_t, base_ptr: nat)
+//   {
+//     && ptr_admissible_16(base_ptr)
+//     && base_ptr in heap
+//     && heap[base_ptr].W16?
+//   }
 
-  function heap_w16_read(heap: heap_t, ptr: nat): uint16
-    requires heap_w16_ptr_valid(heap, ptr)
-  {
-    heap[ptr].w16
-  }
+//   function heap_w16_read(heap: heap_t, ptr: nat): uint16
+//     requires heap_w16_ptr_valid(heap, ptr)
+//   {
+//     heap[ptr].w16
+//   }
 
-  function heap_w16_write(heap: heap_t, ptr: nat, value: uint16): heap_t
-    requires heap_w16_ptr_valid(heap, ptr)
-  {
-    heap[ptr := W16(value)]
-  }
+//   function heap_w16_write(heap: heap_t, ptr: nat, value: uint16): heap_t
+//     requires heap_w16_ptr_valid(heap, ptr)
+//   {
+//     heap[ptr := W16(value)]
+//   }
 
-  // this holds for each W16 heaplet entry
-  predicate heap_w16_inv(heap: heap_t, flat: flat_t, ptr: nat)
-    requires heap_w16_ptr_valid(heap, ptr)
-  {
-    && flat_ptr_valid_16(flat, ptr)
-    && heap[ptr].w16 == flat_read_16(flat, ptr)
-    // disjointness from stack
-    && !in_stack_addr_range(ptr)
-  }
+//   // this holds for each W16 heaplet entry
+//   predicate heap_w16_inv(heap: heap_t, flat: flat_t, ptr: nat)
+//     requires heap_w16_ptr_valid(heap, ptr)
+//   {
+//     && flat_ptr_valid_16(flat, ptr)
+//     && heap[ptr].w16 == flat_read_16(flat, ptr)
+//     // disjointness from stack
+//     && !in_stack_addr_range(ptr)
+//   }
 
-  predicate stack_addrs_valid(flat: flat_t)
-  {
-    forall i | 0 <= i < STACK_MAX_WORDS() ::
-      flat_ptr_valid_16(flat, stack_index_to_ptr(i))
-  }
+//   predicate stack_addrs_valid(flat: flat_t)
+//   {
+//     forall i | 0 <= i < STACK_MAX_WORDS() ::
+//       flat_ptr_valid_16(flat, stack_index_to_ptr(i))
+//   }
 
-  function {:opaque} get_stack(flat: flat_t): (stack: seq<uint16>)
-    requires stack_addrs_valid(flat)
-    ensures |stack| ==  STACK_MAX_WORDS()
-  {
-    seq(STACK_MAX_WORDS(),
-      n requires 0 <= n < STACK_MAX_WORDS() =>
-        flat_read_16(flat, stack_index_to_ptr(n)))
-  }
+//   function {:opaque} get_stack(flat: flat_t): (stack: seq<uint16>)
+//     requires stack_addrs_valid(flat)
+//     ensures |stack| ==  STACK_MAX_WORDS()
+//   {
+//     seq(STACK_MAX_WORDS(),
+//       n requires 0 <= n < STACK_MAX_WORDS() =>
+//         flat_read_16(flat, stack_index_to_ptr(n)))
+//   }
 
-  datatype imem_t = imem_cons(heap: heap_t, stack: seq<uint16>)
-  {
-    predicate stack_inv(flat: flat_t)
-    {
-      && stack_addrs_valid(flat)
-      && stack == get_stack(flat)
-      && (forall i | 0 <= i < STACK_MAX_WORDS() ::
-        stack_index_to_ptr(i) !in heap)
-    }
+//   datatype imem_t = imem_cons(heap: heap_t, stack: seq<uint16>)
+//   {
+//     predicate stack_inv(flat: flat_t)
+//     {
+//       && stack_addrs_valid(flat)
+//       && stack == get_stack(flat)
+//       && (forall i | 0 <= i < STACK_MAX_WORDS() ::
+//         stack_index_to_ptr(i) !in heap)
+//     }
 
-    // the equivalence invariant between heaplet and memory
-    predicate inv(flat: flat_t)
-    {
-      && (forall base_ptr | heap_b16_ptr_valid(heap, base_ptr) ::
-        heap_b16_inv(heap, flat, base_ptr))
-      && (forall base_ptr | heap_w16_ptr_valid(heap, base_ptr) ::
-        heap_w16_inv(heap, flat, base_ptr))
-      && stack_inv(flat)
-    }
+//     // the equivalence invariant between heaplet and memory
+//     predicate inv(flat: flat_t)
+//     {
+//       && (forall base_ptr | heap_b16_ptr_valid(heap, base_ptr) ::
+//         heap_b16_inv(heap, flat, base_ptr))
+//       && (forall base_ptr | heap_w16_ptr_valid(heap, base_ptr) ::
+//         heap_w16_inv(heap, flat, base_ptr))
+//       && stack_inv(flat)
+//     }
 
-    function stack_write(i: nat, value: uint16): imem_t
-      requires i < |stack|
-    {
-      this.(stack := stack[i:= value])
-    }
+//     function stack_write(i: nat, value: uint16): imem_t
+//       requires i < |stack|
+//     {
+//       this.(stack := stack[i:= value])
+//     }
 
-    lemma sub_ptrs_disjoint(flat: flat_t, base1: nat, base2: nat)
-      requires inv(flat)
-      requires heap_b16_ptr_valid(heap, base1)
-      requires heap_b16_ptr_valid(heap, base2)
-      requires base1 != base2
-      ensures forall i, j ::
-        (0 <= i < |heap[base1].b16| && 0 <= j < |heap[base2].b16|)
-          ==> 
-        (heap_b16_index_ptr(base1, i) != heap_b16_index_ptr(base2, j))
-    {
-      var heap := heap;
-      if exists i, j ::
-        && 0 <= i < |heap[base1].b16|
-        && 0 <= j < |heap[base2].b16|
-        && heap_b16_index_ptr(base1, i) == heap_b16_index_ptr(base2, j)
-      {
-        var i, j :|
-          && 0 <= i < |heap[base1].b16|
-          && 0 <= j < |heap[base2].b16|
-          && heap_b16_index_ptr(base1, i) == heap_b16_index_ptr(base2, j);
-        assert base1 + i * 2 == base2 + j * 2;
-        var buff1 := heap[base1].b16;
-        var buff2 := heap[base2].b16;
+//     lemma sub_ptrs_disjoint(flat: flat_t, base1: nat, base2: nat)
+//       requires inv(flat)
+//       requires heap_b16_ptr_valid(heap, base1)
+//       requires heap_b16_ptr_valid(heap, base2)
+//       requires base1 != base2
+//       ensures forall i, j ::
+//         (0 <= i < |heap[base1].b16| && 0 <= j < |heap[base2].b16|)
+//           ==> 
+//         (heap_b16_index_ptr(base1, i) != heap_b16_index_ptr(base2, j))
+//     {
+//       var heap := heap;
+//       if exists i, j ::
+//         && 0 <= i < |heap[base1].b16|
+//         && 0 <= j < |heap[base2].b16|
+//         && heap_b16_index_ptr(base1, i) == heap_b16_index_ptr(base2, j)
+//       {
+//         var i, j :|
+//           && 0 <= i < |heap[base1].b16|
+//           && 0 <= j < |heap[base2].b16|
+//           && heap_b16_index_ptr(base1, i) == heap_b16_index_ptr(base2, j);
+//         assert base1 + i * 2 == base2 + j * 2;
+//         var buff1 := heap[base1].b16;
+//         var buff2 := heap[base2].b16;
 
-        if base1 > base2 {
-          assert heap_b16_inv(heap, flat, base2);
-          var k := j - i;
-          assert base1 == heap_b16_index_ptr(base2, k);
-          assert 0 <= k < |buff2|;
-          assert heap_16_inv(heap, flat, base2, k);
-          assert base1 !in heap;
-          assert false;
-        } else {
-          assert heap_b16_inv(heap, flat, base1);
-          var k := i - j;
-          assert base2 == heap_b16_index_ptr(base1, k);
-          assert 0 <= k < |buff1|;
-          assert heap_16_inv(heap, flat, base1, k);
-          assert base2 !in heap;
-          assert false;
-        }
-      }
-    }
+//         if base1 > base2 {
+//           assert heap_b16_inv(heap, flat, base2);
+//           var k := j - i;
+//           assert base1 == heap_b16_index_ptr(base2, k);
+//           assert 0 <= k < |buff2|;
+//           assert heap_16_inv(heap, flat, base2, k);
+//           assert base1 !in heap;
+//           assert false;
+//         } else {
+//           assert heap_b16_inv(heap, flat, base1);
+//           var k := i - j;
+//           assert base2 == heap_b16_index_ptr(base1, k);
+//           assert 0 <= k < |buff1|;
+//           assert heap_16_inv(heap, flat, base1, k);
+//           assert base2 !in heap;
+//           assert false;
+//         }
+//       }
+//     }
 
-    lemma heap_b16_write_preserves_b16_inv(
-      flat: flat_t, new_flat: flat_t,
-      iter: b16_iter, value: uint16,
-      other_ptr: nat)
+//     lemma heap_b16_write_preserves_b16_inv(
+//       flat: flat_t, new_flat: flat_t,
+//       iter: b16_iter, value: uint16,
+//       other_ptr: nat)
 
-      requires inv(flat)
-      requires b16_iter_safe(heap, iter)
-      requires new_flat == flat_write_16(flat, iter.cur_ptr(), value)
-      requires heap_b16_ptr_valid(heap, other_ptr)
+//       requires inv(flat)
+//       requires b16_iter_safe(heap, iter)
+//       requires new_flat == flat_write_16(flat, iter.cur_ptr(), value)
+//       requires heap_b16_ptr_valid(heap, other_ptr)
 
-      ensures heap_b16_inv(heap_b16_write(heap, iter, value),
-        flat_write_16(flat, iter.cur_ptr(), value), other_ptr)
-    {
-      var new_heap := heap_b16_write(heap, iter, value);
-      var base_ptr, j := iter.base_ptr, iter.index;
-      var buff := heap[other_ptr].b16;
-      var len := |buff|;
+//       ensures heap_b16_inv(heap_b16_write(heap, iter, value),
+//         flat_write_16(flat, iter.cur_ptr(), value), other_ptr)
+//     {
+//       var new_heap := heap_b16_write(heap, iter, value);
+//       var base_ptr, j := iter.base_ptr, iter.index;
+//       var buff := heap[other_ptr].b16;
+//       var len := |buff|;
 
-      if other_ptr == base_ptr {
-        forall i | 0 <= i < len
-          ensures heap_16_inv(new_heap, new_flat, base_ptr, i)
-        {
-          assert heap_16_inv(heap, flat, base_ptr, i);
-          if i == j {
-            value_16_from_16(value);
-            assert heap_16_inv(new_heap, new_flat, base_ptr, i);
-          }
-        }
-      } else {
-        forall i | 0 <= i < len
-          ensures heap_16_inv(new_heap, new_flat, other_ptr, i)
-        {
-          assert heap_16_inv(heap, flat, other_ptr, i);
-          var ptr := heap_b16_index_ptr(other_ptr, i);
-          assert flat_ptr_valid_16(new_flat, ptr);
-          assert ptr != iter.cur_ptr() by {
-            sub_ptrs_disjoint(flat, other_ptr, base_ptr);
-          }
-          assert flat_read_16(new_flat, ptr) == buff[i];
-        }
-      }
-      assert heap_b16_inv(heap, flat, other_ptr);
-    }
+//       if other_ptr == base_ptr {
+//         forall i | 0 <= i < len
+//           ensures heap_16_inv(new_heap, new_flat, base_ptr, i)
+//         {
+//           assert heap_16_inv(heap, flat, base_ptr, i);
+//           if i == j {
+//             value_16_from_16(value);
+//             assert heap_16_inv(new_heap, new_flat, base_ptr, i);
+//           }
+//         }
+//       } else {
+//         forall i | 0 <= i < len
+//           ensures heap_16_inv(new_heap, new_flat, other_ptr, i)
+//         {
+//           assert heap_16_inv(heap, flat, other_ptr, i);
+//           var ptr := heap_b16_index_ptr(other_ptr, i);
+//           assert flat_ptr_valid_16(new_flat, ptr);
+//           assert ptr != iter.cur_ptr() by {
+//             sub_ptrs_disjoint(flat, other_ptr, base_ptr);
+//           }
+//           assert flat_read_16(new_flat, ptr) == buff[i];
+//         }
+//       }
+//       assert heap_b16_inv(heap, flat, other_ptr);
+//     }
 
-    lemma heap_b16_write_preserves_stack_inv(
-      flat: flat_t, new_flat: flat_t,
-      iter: b16_iter, value: uint16)
+//     lemma heap_b16_write_preserves_stack_inv(
+//       flat: flat_t, new_flat: flat_t,
+//       iter: b16_iter, value: uint16)
 
-      requires inv(flat)
-      requires b16_iter_safe(heap, iter)
-      requires new_flat == flat_write_16(flat, iter.cur_ptr(), value)
+//       requires inv(flat)
+//       requires b16_iter_safe(heap, iter)
+//       requires new_flat == flat_write_16(flat, iter.cur_ptr(), value)
 
-      ensures this.(heap := heap_b16_write(heap, iter, value)).stack_inv(new_flat)
-    {
-      var new_heap := heap_b16_write(heap, iter, value);
-      var new_mem := this.(heap := new_heap);
+//       ensures this.(heap := heap_b16_write(heap, iter, value)).stack_inv(new_flat)
+//     {
+//       var new_heap := heap_b16_write(heap, iter, value);
+//       var new_mem := this.(heap := new_heap);
   
-      assert (this.(heap := new_heap)).stack_inv(new_flat) by {
-        forall n | 0 <= n < STACK_MAX_WORDS()
-          ensures flat_read_16(flat, stack_index_to_ptr(n))
-            == 
-          flat_read_16(new_flat, stack_index_to_ptr(n))
-        {
-          var ptr := stack_index_to_ptr(n);
-          if flat[ptr] != new_flat[ptr] {
-            assert heap_16_inv(heap, flat, iter.base_ptr, iter.index);
-            assert false;
-          }
-        }
-        reveal get_stack();
-      }
-    }
+//       assert (this.(heap := new_heap)).stack_inv(new_flat) by {
+//         forall n | 0 <= n < STACK_MAX_WORDS()
+//           ensures flat_read_16(flat, stack_index_to_ptr(n))
+//             == 
+//           flat_read_16(new_flat, stack_index_to_ptr(n))
+//         {
+//           var ptr := stack_index_to_ptr(n);
+//           if flat[ptr] != new_flat[ptr] {
+//             assert heap_16_inv(heap, flat, iter.base_ptr, iter.index);
+//             assert false;
+//           }
+//         }
+//         reveal get_stack();
+//       }
+//     }
 
-    lemma heap_b16_write_preserves_w16_inv(
-      flat: flat_t, new_flat: flat_t,
-      iter: b16_iter, value: uint16, other_ptr: nat)
+//     lemma heap_b16_write_preserves_w16_inv(
+//       flat: flat_t, new_flat: flat_t,
+//       iter: b16_iter, value: uint16, other_ptr: nat)
 
-      requires inv(flat)
-      requires b16_iter_safe(heap, iter)
-      requires new_flat == flat_write_16(flat, iter.cur_ptr(), value)
-      requires heap_w16_ptr_valid(heap, other_ptr)
+//       requires inv(flat)
+//       requires b16_iter_safe(heap, iter)
+//       requires new_flat == flat_write_16(flat, iter.cur_ptr(), value)
+//       requires heap_w16_ptr_valid(heap, other_ptr)
 
-      ensures heap_w16_inv(heap_b16_write(heap, iter, value), new_flat, other_ptr)
-    {
-      if flat[other_ptr] != new_flat[other_ptr] {
-        assert heap_16_inv(heap, flat, iter.base_ptr, iter.index);
-        assert false;
-      }
-    }
+//       ensures heap_w16_inv(heap_b16_write(heap, iter, value), new_flat, other_ptr)
+//     {
+//       if flat[other_ptr] != new_flat[other_ptr] {
+//         assert heap_16_inv(heap, flat, iter.base_ptr, iter.index);
+//         assert false;
+//       }
+//     }
   
-    lemma heap_b16_write_preverses_inv(
-      flat: flat_t, new_flat: flat_t,
-      iter: b16_iter, value: uint16)
+//     lemma heap_b16_write_preverses_inv(
+//       flat: flat_t, new_flat: flat_t,
+//       iter: b16_iter, value: uint16)
 
-      requires inv(flat)
-      requires b16_iter_safe(heap, iter)
-      requires new_flat == flat_write_16(flat, iter.cur_ptr(), value)
+//       requires inv(flat)
+//       requires b16_iter_safe(heap, iter)
+//       requires new_flat == flat_write_16(flat, iter.cur_ptr(), value)
 
-      ensures this.(heap := heap_b16_write(heap, iter, value)).inv(new_flat)
-    {
-      var new_heap := heap_b16_write(heap, iter, value);
-      var new_mem := this.(heap := new_heap);
+//       ensures this.(heap := heap_b16_write(heap, iter, value)).inv(new_flat)
+//     {
+//       var new_heap := heap_b16_write(heap, iter, value);
+//       var new_mem := this.(heap := new_heap);
 
-      forall base_ptr | heap_b16_ptr_valid(new_heap, base_ptr)
-        ensures heap_b16_inv(new_heap, new_flat, base_ptr)
-      {
-        heap_b16_write_preserves_b16_inv(flat, new_flat, iter, value, base_ptr);
-      }
-      forall base_ptr | heap_w16_ptr_valid(new_heap, base_ptr)
-        ensures heap_w16_inv(new_heap, new_flat, base_ptr)
-      {
-        heap_b16_write_preserves_w16_inv(flat, new_flat, iter, value, base_ptr);
-      }
+//       forall base_ptr | heap_b16_ptr_valid(new_heap, base_ptr)
+//         ensures heap_b16_inv(new_heap, new_flat, base_ptr)
+//       {
+//         heap_b16_write_preserves_b16_inv(flat, new_flat, iter, value, base_ptr);
+//       }
+//       forall base_ptr | heap_w16_ptr_valid(new_heap, base_ptr)
+//         ensures heap_w16_inv(new_heap, new_flat, base_ptr)
+//       {
+//         heap_b16_write_preserves_w16_inv(flat, new_flat, iter, value, base_ptr);
+//       }
 
-      heap_b16_write_preserves_stack_inv(
-        flat, new_flat, iter, value);
-    }
+//       heap_b16_write_preserves_stack_inv(
+//         flat, new_flat, iter, value);
+//     }
 
-    lemma heap_w16_write_preserves_b16_inv(
-      flat: flat_t, new_flat: flat_t,
-      write_ptr: nat, value: uint16, other_ptr: nat)
+//     lemma heap_w16_write_preserves_b16_inv(
+//       flat: flat_t, new_flat: flat_t,
+//       write_ptr: nat, value: uint16, other_ptr: nat)
 
-      requires inv(flat)
-      requires heap_w16_ptr_valid(heap, write_ptr)
-      requires new_flat == flat_write_16(flat, write_ptr, value)
+//       requires inv(flat)
+//       requires heap_w16_ptr_valid(heap, write_ptr)
+//       requires new_flat == flat_write_16(flat, write_ptr, value)
 
-      requires heap_b16_ptr_valid(heap, other_ptr)
+//       requires heap_b16_ptr_valid(heap, other_ptr)
 
-      ensures heap_b16_inv(heap_w16_write(heap, write_ptr, value), new_flat, other_ptr)
-    {
-      var new_heap := heap_w16_write(heap, write_ptr, value);
-      assert heap_b16_inv(heap, flat, other_ptr);
-      var buff := heap[other_ptr].b16;
-      forall i | 0 <= i < |buff| 
-        ensures heap_16_inv(new_heap, new_flat, other_ptr, i)
-      {
-        assert heap_16_inv(heap, flat, other_ptr, i);
-      }
-    }
+//       ensures heap_b16_inv(heap_w16_write(heap, write_ptr, value), new_flat, other_ptr)
+//     {
+//       var new_heap := heap_w16_write(heap, write_ptr, value);
+//       assert heap_b16_inv(heap, flat, other_ptr);
+//       var buff := heap[other_ptr].b16;
+//       forall i | 0 <= i < |buff| 
+//         ensures heap_16_inv(new_heap, new_flat, other_ptr, i)
+//       {
+//         assert heap_16_inv(heap, flat, other_ptr, i);
+//       }
+//     }
 
-    lemma heap_w16_write_preserves_w16_inv(
-      flat: flat_t, new_flat: flat_t,
-      write_ptr: nat, value: uint16, other_ptr: nat)
+//     lemma heap_w16_write_preserves_w16_inv(
+//       flat: flat_t, new_flat: flat_t,
+//       write_ptr: nat, value: uint16, other_ptr: nat)
 
-      requires inv(flat)
-      requires heap_w16_ptr_valid(heap, write_ptr)
-      requires new_flat == flat_write_16(flat, write_ptr, value)
+//       requires inv(flat)
+//       requires heap_w16_ptr_valid(heap, write_ptr)
+//       requires new_flat == flat_write_16(flat, write_ptr, value)
 
-      requires heap_w16_ptr_valid(heap, other_ptr)
+//       requires heap_w16_ptr_valid(heap, other_ptr)
 
-      ensures heap_w16_inv(heap_w16_write(heap, write_ptr, value), new_flat, other_ptr)
-    {
-      if other_ptr == write_ptr {
-        value_16_from_16(value);
-      }
-    }
+//       ensures heap_w16_inv(heap_w16_write(heap, write_ptr, value), new_flat, other_ptr)
+//     {
+//       if other_ptr == write_ptr {
+//         value_16_from_16(value);
+//       }
+//     }
 
-    lemma heap_w16_write_preserves_stack_inv(
-      flat: flat_t, new_flat: flat_t,
-      value: uint16, write_ptr: nat)
+//     lemma heap_w16_write_preserves_stack_inv(
+//       flat: flat_t, new_flat: flat_t,
+//       value: uint16, write_ptr: nat)
 
-      requires inv(flat)
-      requires heap_w16_ptr_valid(heap, write_ptr)
-      requires new_flat == flat_write_16(flat, write_ptr, value)
+//       requires inv(flat)
+//       requires heap_w16_ptr_valid(heap, write_ptr)
+//       requires new_flat == flat_write_16(flat, write_ptr, value)
 
-      ensures this.(heap := heap_w16_write(heap, write_ptr, value)).stack_inv(new_flat)
-    {
-      var new_heap := heap_w16_write(heap, write_ptr, value);
+//       ensures this.(heap := heap_w16_write(heap, write_ptr, value)).stack_inv(new_flat)
+//     {
+//       var new_heap := heap_w16_write(heap, write_ptr, value);
   
-      assert (this.(heap := new_heap)).stack_inv(new_flat) by {
-        reveal get_stack();
-      }
-    }
+//       assert (this.(heap := new_heap)).stack_inv(new_flat) by {
+//         reveal get_stack();
+//       }
+//     }
 
-    lemma heap_w16_write_preverses_inv(
-      flat: flat_t, new_flat: flat_t,
-      write_ptr: nat, value: uint16)
+//     lemma heap_w16_write_preverses_inv(
+//       flat: flat_t, new_flat: flat_t,
+//       write_ptr: nat, value: uint16)
 
-      requires inv(flat)
-      requires heap_w16_ptr_valid(heap, write_ptr)
-      requires new_flat == flat_write_16(flat, write_ptr, value)
+//       requires inv(flat)
+//       requires heap_w16_ptr_valid(heap, write_ptr)
+//       requires new_flat == flat_write_16(flat, write_ptr, value)
 
-      ensures this.(heap := heap_w16_write(heap, write_ptr, value)).inv(new_flat)
-    {
-      var new_heap := heap_w16_write(heap, write_ptr, value);
+//       ensures this.(heap := heap_w16_write(heap, write_ptr, value)).inv(new_flat)
+//     {
+//       var new_heap := heap_w16_write(heap, write_ptr, value);
 
-      forall base_ptr | heap_b16_ptr_valid(new_heap, base_ptr)
-        ensures heap_b16_inv(new_heap, new_flat, base_ptr)
-      {
-        heap_w16_write_preserves_b16_inv(flat, new_flat, write_ptr, value, base_ptr);
-      }
-      forall base_ptr | heap_w16_ptr_valid(new_heap, base_ptr)
-        ensures heap_w16_inv(new_heap, new_flat, base_ptr)
-      {
-        heap_w16_write_preserves_w16_inv(flat, new_flat, write_ptr, value, base_ptr);
-      }
-      heap_w16_write_preserves_stack_inv(flat, new_flat, value, write_ptr);
-    }
+//       forall base_ptr | heap_b16_ptr_valid(new_heap, base_ptr)
+//         ensures heap_b16_inv(new_heap, new_flat, base_ptr)
+//       {
+//         heap_w16_write_preserves_b16_inv(flat, new_flat, write_ptr, value, base_ptr);
+//       }
+//       forall base_ptr | heap_w16_ptr_valid(new_heap, base_ptr)
+//         ensures heap_w16_inv(new_heap, new_flat, base_ptr)
+//       {
+//         heap_w16_write_preserves_w16_inv(flat, new_flat, write_ptr, value, base_ptr);
+//       }
+//       heap_w16_write_preserves_stack_inv(flat, new_flat, value, write_ptr);
+//     }
 
-    lemma stack_write_preserves_b16_inv(
-      flat: flat_t, new_flat: flat_t,
-      index: nat, value: uint16, base_ptr: nat)
+//     lemma stack_write_preserves_b16_inv(
+//       flat: flat_t, new_flat: flat_t,
+//       index: nat, value: uint16, base_ptr: nat)
 
-      requires inv(flat)
-      requires index < |stack|
-      requires new_flat == flat_write_16(flat, stack_index_to_ptr(index), value)
-      requires heap_b16_ptr_valid(heap, base_ptr)
+//       requires inv(flat)
+//       requires index < |stack|
+//       requires new_flat == flat_write_16(flat, stack_index_to_ptr(index), value)
+//       requires heap_b16_ptr_valid(heap, base_ptr)
   
-      ensures heap_b16_inv(heap, new_flat, base_ptr)
-    {
-      var buff := heap[base_ptr].b16;
-      var new_buff := heap[base_ptr].b16;
+//       ensures heap_b16_inv(heap, new_flat, base_ptr)
+//     {
+//       var buff := heap[base_ptr].b16;
+//       var new_buff := heap[base_ptr].b16;
   
-      forall i | 0 <= i < |new_buff|
-        ensures heap_16_inv(heap, new_flat, base_ptr, i) 
-      {
-        assert heap_16_inv(heap, flat, base_ptr, i);
-      }
-    }
+//       forall i | 0 <= i < |new_buff|
+//         ensures heap_16_inv(heap, new_flat, base_ptr, i) 
+//       {
+//         assert heap_16_inv(heap, flat, base_ptr, i);
+//       }
+//     }
 
-    lemma stack_write_preserves_w16_inv(
-      flat: flat_t, new_flat: flat_t,
-      index: nat, value: uint16,
-      other_ptr: nat)
+//     lemma stack_write_preserves_w16_inv(
+//       flat: flat_t, new_flat: flat_t,
+//       index: nat, value: uint16,
+//       other_ptr: nat)
 
-      requires inv(flat)
-      requires index < |stack|
-      requires new_flat == flat_write_16(flat, stack_index_to_ptr(index), value)
-      requires heap_w16_ptr_valid(heap, other_ptr)
+//       requires inv(flat)
+//       requires index < |stack|
+//       requires new_flat == flat_write_16(flat, stack_index_to_ptr(index), value)
+//       requires heap_w16_ptr_valid(heap, other_ptr)
 
-      ensures heap_w16_inv(heap, new_flat, other_ptr)
-    {
-    }
+//       ensures heap_w16_inv(heap, new_flat, other_ptr)
+//     {
+//     }
 
-    lemma stack_write_preserves_stack_inv(
-      flat: flat_t, new_flat: flat_t,
-      index: nat, value: uint16)
+//     lemma stack_write_preserves_stack_inv(
+//       flat: flat_t, new_flat: flat_t,
+//       index: nat, value: uint16)
 
-      requires inv(flat)
-      requires index < |stack|
-      requires new_flat == flat_write_16(flat, stack_index_to_ptr(index), value)
+//       requires inv(flat)
+//       requires index < |stack|
+//       requires new_flat == flat_write_16(flat, stack_index_to_ptr(index), value)
   
-      ensures this.(stack := stack[index := value]).stack_inv(new_flat)
-    {
-      var new_stack := stack[index := value];
-      reveal get_stack();
-      value_16_from_16(value);
-      assert get_stack(new_flat) == new_stack;
-    }
+//       ensures this.(stack := stack[index := value]).stack_inv(new_flat)
+//     {
+//       var new_stack := stack[index := value];
+//       reveal get_stack();
+//       value_16_from_16(value);
+//       assert get_stack(new_flat) == new_stack;
+//     }
 
-    lemma stack_write_preverses_inv(
-      flat: flat_t, new_flat: flat_t,
-      index: nat, value: uint16)
+//     lemma stack_write_preverses_inv(
+//       flat: flat_t, new_flat: flat_t,
+//       index: nat, value: uint16)
 
-      requires inv(flat)
-      requires index < |stack|
-      requires new_flat == flat_write_16(flat, stack_index_to_ptr(index), value)
+//       requires inv(flat)
+//       requires index < |stack|
+//       requires new_flat == flat_write_16(flat, stack_index_to_ptr(index), value)
 
-      ensures this.(stack := stack[index := value]).inv(new_flat)
-    {
-      forall base_ptr | heap_b16_ptr_valid(heap, base_ptr)
-        ensures heap_b16_inv(heap, new_flat, base_ptr)
-      {
-        stack_write_preserves_b16_inv(flat, new_flat, index, value, base_ptr);
-      }
+//       ensures this.(stack := stack[index := value]).inv(new_flat)
+//     {
+//       forall base_ptr | heap_b16_ptr_valid(heap, base_ptr)
+//         ensures heap_b16_inv(heap, new_flat, base_ptr)
+//       {
+//         stack_write_preserves_b16_inv(flat, new_flat, index, value, base_ptr);
+//       }
       
-      forall base_ptr | heap_w16_ptr_valid(heap, base_ptr)
-        ensures heap_w16_inv(heap, new_flat, base_ptr)
-      {
-        stack_write_preserves_w16_inv(flat, new_flat, index, value, base_ptr);
-      }
+//       forall base_ptr | heap_w16_ptr_valid(heap, base_ptr)
+//         ensures heap_w16_inv(heap, new_flat, base_ptr)
+//       {
+//         stack_write_preserves_w16_inv(flat, new_flat, index, value, base_ptr);
+//       }
     
-      stack_write_preserves_stack_inv(flat, new_flat,
-        index, value);
-    }
-  }
+//       stack_write_preserves_stack_inv(flat, new_flat,
+//         index, value);
+//     }
+//   }
 
-  datatype mem_t = mem_cons(heap: heap_t, frames: frames_t, symbols: map<string, uint16>)
-  {
-    function as_imem(flat: flat_t): imem_t
-      requires stack_addrs_valid(flat)
-    {
-      imem_cons(heap, get_stack(flat))
-    }
+//   datatype mem_t = mem_cons(heap: heap_t, frames: frames_t, symbols: map<string, uint16>)
+//   {
+//     function as_imem(flat: flat_t): imem_t
+//       requires stack_addrs_valid(flat)
+//     {
+//       imem_cons(heap, get_stack(flat))
+//     }
 
-    predicate {:opaque} inv(flat: flat_t)
-      ensures inv(flat) ==> symbols_inv()
-      ensures inv(flat) ==> |frames.fs| >= 1
-    {
-      && stack_addrs_valid(flat)
-      && as_imem(flat).inv(flat)
-      && frames.frames_inv(get_stack(flat))
-      && symbols_inv()
-    }
+//     predicate {:opaque} inv(flat: flat_t)
+//       ensures inv(flat) ==> symbols_inv()
+//       ensures inv(flat) ==> |frames.fs| >= 1
+//     {
+//       && stack_addrs_valid(flat)
+//       && as_imem(flat).inv(flat)
+//       && frames.frames_inv(get_stack(flat))
+//       && symbols_inv()
+//     }
 
-    predicate {:opaque} symbols_inv()
-    {
-      forall name: string :: 
-        name in symbols ==> ptr_admissible_16(symbols[name])
-    }
+//     predicate {:opaque} symbols_inv()
+//     {
+//       forall name: string :: 
+//         name in symbols ==> ptr_admissible_16(symbols[name])
+//     }
 
-    function load_symbol(name: string): uint16
-      requires name in symbols
-      requires symbols_inv()
-    {
-      reveal symbols_inv();
-      symbols[name]
-    }
+//     function load_symbol(name: string): uint16
+//       requires name in symbols
+//       requires symbols_inv()
+//     {
+//       reveal symbols_inv();
+//       symbols[name]
+//     }
 
-    lemma heap_b16_write_preverses_inv(
-      flat: flat_t, iter: b16_iter, value: uint16)
+//     lemma heap_b16_write_preverses_inv(
+//       flat: flat_t, iter: b16_iter, value: uint16)
 
-      requires inv(flat)
-      requires b16_iter_safe(heap, iter)
+//       requires inv(flat)
+//       requires b16_iter_safe(heap, iter)
 
-      ensures this.(heap := heap_b16_write(heap, iter, value)).
-        inv(flat_write_16(flat, iter.cur_ptr(), value))
-    {
-      reveal inv();
-      reveal symbols_inv();
-      var new_flat := flat_write_16(flat, iter.cur_ptr(), value);
-      as_imem(flat).heap_b16_write_preverses_inv(flat, new_flat,
-        iter, value);
-    }
+//       ensures this.(heap := heap_b16_write(heap, iter, value)).
+//         inv(flat_write_16(flat, iter.cur_ptr(), value))
+//     {
+//       reveal inv();
+//       reveal symbols_inv();
+//       var new_flat := flat_write_16(flat, iter.cur_ptr(), value);
+//       as_imem(flat).heap_b16_write_preverses_inv(flat, new_flat,
+//         iter, value);
+//     }
 
-    lemma heap_w16_write_preverses_inv(
-      flat: flat_t, write_ptr: nat, value: uint16)
+//     lemma heap_w16_write_preverses_inv(
+//       flat: flat_t, write_ptr: nat, value: uint16)
     
-      requires inv(flat)
-      requires heap_w16_ptr_valid(heap, write_ptr)
-      ensures this.(heap := heap_w16_write(heap, write_ptr, value)).
-        inv(flat_write_16(flat, write_ptr, value))
-    {
-      reveal inv();
-      reveal symbols_inv();
-      var new_flat := flat_write_16(flat, write_ptr, value);
-      as_imem(flat).heap_w16_write_preverses_inv(flat, new_flat,
-        write_ptr, value);
-    }
+//       requires inv(flat)
+//       requires heap_w16_ptr_valid(heap, write_ptr)
+//       ensures this.(heap := heap_w16_write(heap, write_ptr, value)).
+//         inv(flat_write_16(flat, write_ptr, value))
+//     {
+//       reveal inv();
+//       reveal symbols_inv();
+//       var new_flat := flat_write_16(flat, write_ptr, value);
+//       as_imem(flat).heap_w16_write_preverses_inv(flat, new_flat,
+//         write_ptr, value);
+//     }
 
-    lemma frames_write_preverses_inv(flat: flat_t, index: nat, value: uint16)
-      requires inv(flat)
-      requires frames.write.requires(index, value)
+//     lemma frames_write_preverses_inv(flat: flat_t, index: nat, value: uint16)
+//       requires inv(flat)
+//       requires frames.write.requires(index, value)
 
-      ensures in_stack_addr_range(frames.sp + index * 2)
-      ensures this.(frames := frames.write(index, value)).
-        inv(flat_write_16(flat, frames.sp + index * 2, value))
-    {
-      reveal inv();
-      reveal symbols_inv();
+//       ensures in_stack_addr_range(frames.sp + index * 2)
+//       ensures this.(frames := frames.write(index, value)).
+//         inv(flat_write_16(flat, frames.sp + index * 2, value))
+//     {
+//       reveal inv();
+//       reveal symbols_inv();
 
-      var new_mem := this.(frames := frames.write(index, value));
-      var stack_index := ptr_to_stack_index(frames.sp) + index;
-      var write_ptr := stack_index_to_ptr(stack_index);
+//       var new_mem := this.(frames := frames.write(index, value));
+//       var stack_index := ptr_to_stack_index(frames.sp) + index;
+//       var write_ptr := stack_index_to_ptr(stack_index);
 
-      calc == {
-        write_ptr;
-        STACK_END() + (ptr_to_stack_index(frames.sp) + index) * 2;
-        {
-          Mul.LemmaMulIsDistributiveAddAuto();
-        }
-        STACK_END() + ptr_to_stack_index(frames.sp) * 2 + index * 2;
-        STACK_END() + ((frames.sp - STACK_END()) / 2) * 2 + index * 2;
-        {
-          assert DivMod.IsModEquivalent(frames.sp, STACK_END(),2);  // pain
-          LemmaDivMulNop(frames.sp - STACK_END(),2); 
-        }
-        frames.sp + index * 2;
-      }
+//       calc == {
+//         write_ptr;
+//         STACK_END() + (ptr_to_stack_index(frames.sp) + index) * 2;
+//         {
+//           Mul.LemmaMulIsDistributiveAddAuto();
+//         }
+//         STACK_END() + ptr_to_stack_index(frames.sp) * 2 + index * 2;
+//         STACK_END() + ((frames.sp - STACK_END()) / 2) * 2 + index * 2;
+//         {
+//           assert DivMod.IsModEquivalent(frames.sp, STACK_END(),2);  // pain
+//           LemmaDivMulNop(frames.sp - STACK_END(),2); 
+//         }
+//         frames.sp + index * 2;
+//       }
 
-      var new_flat := flat_write_16(flat, frames.sp + index * 2, value);
-      var stack := get_stack(flat);
+//       var new_flat := flat_write_16(flat, frames.sp + index * 2, value);
+//       var stack := get_stack(flat);
 
-      frames.write_preserves_inv(stack, index, value);
+//       frames.write_preserves_inv(stack, index, value);
 
-      assert new_mem.frames.
-        frames_inv(stack[stack_index := value]);
+//       assert new_mem.frames.
+//         frames_inv(stack[stack_index := value]);
 
-      as_imem(flat).stack_write_preverses_inv(flat, new_flat,
-        stack_index, value);
+//       as_imem(flat).stack_write_preverses_inv(flat, new_flat,
+//         stack_index, value);
 
-      assert as_imem(flat).(stack := stack[stack_index := value]).inv(new_flat);
-    }
-  }
+//       assert as_imem(flat).(stack := stack[stack_index := value]).inv(new_flat);
+//     }
+//   }
 
-  function stack_depth(mem: mem_t): nat
-  {
-    mem.frames.depth()
-  }
+//   function stack_depth(mem: mem_t): nat
+//   {
+//     mem.frames.depth()
+//   }
 
-  function {:opaque} stack_push_frame(mem: mem_t, flat: flat_t, num_bytes: uint16): (new_mem: mem_t)
-    requires mem.inv(flat)
-    requires num_bytes % 2 == 0
-    requires in_stack_addr_range(mem.frames.sp - num_bytes)
-    ensures new_mem.inv(flat)
-    ensures frames_top_diff(mem.frames, new_mem.frames)
-    ensures |top_frame(new_mem.frames).content| == num_bytes / 2
-    ensures new_mem== mem.(frames := new_mem.frames)
-  {
-    reveal mem.inv();
-    reveal mem.symbols_inv();
-    var stack := get_stack(flat);
-    mem.frames.push_preserves_inv(num_bytes, stack);
-    var new_mem := mem.(frames := mem.frames.push(num_bytes, stack));
-    assert new_mem.inv(flat);
-    new_mem
-  }
+//   function {:opaque} stack_push_frame(mem: mem_t, flat: flat_t, num_bytes: uint16): (new_mem: mem_t)
+//     requires mem.inv(flat)
+//     requires num_bytes % 2 == 0
+//     requires in_stack_addr_range(mem.frames.sp - num_bytes)
+//     ensures new_mem.inv(flat)
+//     ensures frames_top_diff(mem.frames, new_mem.frames)
+//     ensures |top_frame(new_mem.frames).content| == num_bytes / 2
+//     ensures new_mem== mem.(frames := new_mem.frames)
+//   {
+//     reveal mem.inv();
+//     reveal mem.symbols_inv();
+//     var stack := get_stack(flat);
+//     mem.frames.push_preserves_inv(num_bytes, stack);
+//     var new_mem := mem.(frames := mem.frames.push(num_bytes, stack));
+//     assert new_mem.inv(flat);
+//     new_mem
+//   }
 
-  function stack_pop_frame(mem: mem_t, flat: flat_t): (new_mem: mem_t)
-    requires mem.inv(flat)
-    requires stack_depth(mem) >= 2
-    ensures new_mem.inv(flat)
-    ensures stack_depth(new_mem) == stack_depth(mem) - 1
-  {
-    reveal mem.inv();
-    reveal mem.symbols_inv();
-    var stack := get_stack(flat);
-    mem.frames.pop_preserves_inv(stack);
-    var new_mem := mem.(frames := mem.frames.pop(stack));
-    assert new_mem.inv(flat);
-    new_mem
-  }
+//   function stack_pop_frame(mem: mem_t, flat: flat_t): (new_mem: mem_t)
+//     requires mem.inv(flat)
+//     requires stack_depth(mem) >= 2
+//     ensures new_mem.inv(flat)
+//     ensures stack_depth(new_mem) == stack_depth(mem) - 1
+//   {
+//     reveal mem.inv();
+//     reveal mem.symbols_inv();
+//     var stack := get_stack(flat);
+//     mem.frames.pop_preserves_inv(stack);
+//     var new_mem := mem.(frames := mem.frames.pop(stack));
+//     assert new_mem.inv(flat);
+//     new_mem
+//   }
 
-  function stack_push_batch(mem: mem_t, flat: flat_t, content: seq<uint16>): (new_mem: mem_t)
-  {
-    mem.(frames := mem.frames.push_batch(content))
-  }
+//   function stack_push_batch(mem: mem_t, flat: flat_t, content: seq<uint16>): (new_mem: mem_t)
+//   {
+//     mem.(frames := mem.frames.push_batch(content))
+//   }
 
-  predicate frame_index_valid(mem: mem_t, index: nat)
-  {
-    frames_writable(mem.frames, index)
-  }
+//   predicate frame_index_valid(mem: mem_t, index: nat)
+//   {
+//     frames_writable(mem.frames, index)
+//   }
 
-  function read_top_frame(mem: mem_t): seq<uint16>
-  {
-    if |mem.frames.fs| != 0 then top_frame(mem.frames).content
-    else []
-  }
+//   function read_top_frame(mem: mem_t): seq<uint16>
+//   {
+//     if |mem.frames.fs| != 0 then top_frame(mem.frames).content
+//     else []
+//   }
 
-  function write_frame(mem: mem_t, flat: flat_t, index: nat, value: uint16): (r: (mem_t, flat_t))
-    requires mem.inv(flat)
-    requires frame_index_valid(mem, index)
-    ensures in_stack_addr_range(mem.frames.sp + index * 2)
-    ensures r.1 == flat_write_16(flat, mem.frames.sp + index * 2, value)
-    ensures r.0.inv(r.1)
-    ensures read_top_frame(r.0) == read_top_frame(mem)[index := value];
-  {
-    mem.frames_write_preverses_inv(flat, index, value);
-    var new_mem := mem.(frames := mem.frames.write(index, value));
-    var new_flat := flat_write_16(flat, mem.frames.sp + index * 2, value);
-    (new_mem, new_flat)
-  }
+//   function write_frame(mem: mem_t, flat: flat_t, index: nat, value: uint16): (r: (mem_t, flat_t))
+//     requires mem.inv(flat)
+//     requires frame_index_valid(mem, index)
+//     ensures in_stack_addr_range(mem.frames.sp + index * 2)
+//     ensures r.1 == flat_write_16(flat, mem.frames.sp + index * 2, value)
+//     ensures r.0.inv(r.1)
+//     ensures read_top_frame(r.0) == read_top_frame(mem)[index := value];
+//   {
+//     mem.frames_write_preverses_inv(flat, index, value);
+//     var new_mem := mem.(frames := mem.frames.write(index, value));
+//     var new_flat := flat_write_16(flat, mem.frames.sp + index * 2, value);
+//     (new_mem, new_flat)
+//   }
 
-  function read_frame(mem: mem_t, flat: flat_t, index: nat): (value: uint16)
-    requires mem.inv(flat)
-    requires frame_index_valid(mem, index)
-    // ensures value == flat_read_16(flat, mem.frames.sp + index * 2)
-  {
-    mem.frames.read(index)
-  }
+//   function read_frame(mem: mem_t, flat: flat_t, index: nat): (value: uint16)
+//     requires mem.inv(flat)
+//     requires frame_index_valid(mem, index)
+//     // ensures value == flat_read_16(flat, mem.frames.sp + index * 2)
+//   {
+//     mem.frames.read(index)
+//   }
 
-  function load_symbol(mem: mem_t, name: string): (value: uint16)
-    requires name in mem.symbols
-    requires mem.symbols_inv()
-  {
-    mem.load_symbol(name)
-  }
-}
+//   function load_symbol(mem: mem_t, name: string): (value: uint16)
+//     requires name in mem.symbols
+//     requires mem.symbols_inv()
+//   {
+//     mem.load_symbol(name)
+//   }
+// }
